Introduce more abstractions for world ghost theory + use `open_world_interp_permanent`

theories/model/world_ghost_theory.v
@@ -15,6 +15,8 @@ Section world_ghost_theory.
   .
   Notation E := (WORLD -n> (leibnizO CmptName) -n> (leibnizO Word) -n> iPropO Σ).
   Notation V := (WORLD -n> (leibnizO CmptName) -n> (leibnizO Word) -n> iPropO Σ).
+  Notation Vc := (WORLD * CmptName * Word → iProp Σ).
+
   Implicit Types W : WORLD.
   Implicit Types C : CmptName.
 
@@ -30,13 +32,63 @@ Section world_ghost_theory.
   Definition world_interp_open := proj1_sig world_interp_open_aux.
   Definition world_interp_open_eq : @world_interp_open = @world_interp_open_def := proj2_sig world_interp_open_aux.
 
-  Definition TmpRes (W : WORLD) (C : CmptName) (a : Addr) (p : Perm) Φ (w : Word) : iProp Σ :=
-    ⌜ isO p = false ⌝ ∗ a ↦ₐ w ∗ Φ (W,C,w) ∗
+  Definition mono_temporary (C : CmptName) (p : Perm) (Φ : Vc) (w : Word) : iProp Σ :=
     if (decide ( isWL p = true ∨ isDL p = true )) then future_pub_mono C Φ w else future_priv_mono C Φ w.
+  Definition mono_permanent (C : CmptName) (Φ : Vc) (w : Word) : iProp Σ :=
+    future_priv_mono C Φ w.
+  Definition mono_invariant (C : CmptName) (p : Perm) (Φ : Vc) (w : Word) (ρ : region_type) : iProp Σ :=
+    (if (decide (ρ = Temporary))
+     then mono_temporary C p Φ w
+     else mono_permanent C Φ w).
+
+  Lemma mono_temporary_eq (C : CmptName) (p : Perm) (Φ : Vc) (w : Word) :
+    mono_temporary C p Φ w
+    ⊣⊢ (if isWL p
+        then future_pub_mono C Φ w
+        else if isDL p then future_pub_mono C Φ w else future_priv_mono C Φ w).
+  Proof.
+    rewrite /mono_temporary.
+    destruct isWL; cbn.
+    - case_decide; first done.
+      exfalso; apply H; by left.
+    - destruct isDL; cbn.
+      + case_decide; first done.
+        exfalso; apply H; by right.
+      + case_decide; last done.
+        destruct H; done.
+  Qed.
+
+  Lemma mono_invariant_eq (C : CmptName) (p : Perm) (Φ : Vc) (w : Word) (ρ : region_type) :
+    mono_invariant C p Φ w ρ
+    ⊣⊢
+      (if decide (ρ = Temporary)
+       then
+         if isWL p
+         then future_pub_mono C Φ w
+         else if isDL p then future_pub_mono C Φ w else future_priv_mono C Φ w
+       else future_priv_mono C Φ w).
+  Proof.
+    rewrite /mono_invariant.
+    case_decide as Hρ;auto.
+    apply mono_temporary_eq.
+  Qed.
+
+  Definition TmpRes (W : WORLD) (C : CmptName) (a : Addr) (p : Perm) Φ (w : Word) : iProp Σ :=
+    ⌜ isO p = false ⌝ ∗ a ↦ₐ w ∗ Φ (W,C,w) ∗ mono_temporary C p Φ w.
 
   Definition PermRes (W : WORLD) (C : CmptName) (a : Addr) (p : Perm) Φ (w : Word) : iProp Σ :=
-    ⌜ isO p = false ⌝ ∗ a ↦ₐ w ∗ Φ (W,C,w) ∗ future_priv_mono C Φ w.
+    ⌜ isO p = false ⌝ ∗ a ↦ₐ w ∗ Φ (W,C,w) ∗ mono_permanent C Φ w.
 
+  Definition WorldRes
+    (W : WORLD) (C : CmptName)
+    (a : Addr) (p : Perm) Φ (w : Word) (ρ : region_type) : iProp Σ :=
+    ⌜ isO p = false ⌝ ∗ a ↦ₐ w ∗ Φ (W,C,w) ∗ mono_invariant C p Φ w ρ.
+
+  (* TODO that is "essentially" close_list_resources,
+     defined in regions_invariant_revocation.v,
+     only missing is_later.
+     This is essentially like RevokedResources in logrel_extra.v
+   *)
   Definition RevokedRes (W : WORLD) (C : CmptName) (s : list Addr) : iProp Σ :=
     [∗ list] a ∈ s, (∃ pa Φa, ⌜∀ WCv, Persistent (Φa WCv)⌝ ∗ rel C a pa Φa ∗ ∃ wa, TmpRes W C a pa Φa wa).
 
@@ -48,7 +100,8 @@ Section world_ghost_theory.
     (W : WORLD) (C : CmptName) (a : Addr) (p : Perm) (P : V) :
     (std W) !! a = Some Permanent ∨ (std W) !! a = Some Temporary ->
     world_interp W C -∗
-    rel C a p (safeC P) ==∗
+    rel C a p (safeC P)
+    ==∗
     ∃ w, a ↦ₐ w ∗ ▷ P W C w.
   Proof.
     rewrite world_interp_eq /world_interp_def.
@@ -77,7 +130,11 @@ Section world_ghost_theory.
       iFrame.
   Qed.
 
-  Lemma open_empty (W : WORLD) (C : CmptName) :
+  Lemma world_interp_init (W : WORLD) (C : CmptName) :
+    region W C ∗ sts_full_world W C -∗ world_interp W C.
+  Proof. rewrite world_interp_eq /world_interp_def; iIntros "[? ?]"; iFrame. Qed.
+
+  Lemma open_world_interp_empty (W : WORLD) (C : CmptName) :
     world_interp_open W C [] ⊣⊢ world_interp W C.
   Proof.
     rewrite world_interp_eq /world_interp_def.
@@ -86,13 +143,15 @@ Section world_ghost_theory.
     iSplit ; iIntros "[Hr $]"; iApply region_open_nil; done.
   Qed.
 
-  Lemma open_temporary (W : WORLD) (C : CmptName) (s : list Addr) (a : Addr) (p : Perm) Φ :
+  Lemma open_world_interp_temporary (W : WORLD) (C : CmptName) (s : list Addr) (a : Addr) (p : Perm) Φ :
     a ∉ s ->
     (std W) !! a = Some Temporary ->
     world_interp_open W C s -∗
     rel C a p Φ
     -∗
-    world_interp_open W C ({[ a ]} ∪ s) ∗ sts_state_std C a Temporary ∗ ▷ (∃ w, TmpRes W C a p Φ w).
+    world_interp_open W C ({[ a ]} ∪ s) ∗
+    sts_state_std C a Temporary ∗
+    ▷ (∃ w, TmpRes W C a p Φ w).
   Proof.
     rewrite world_interp_open_eq /world_interp_open_def.
     iIntros (Ha HWa) "[Hr Hsts] Hrel".
@@ -100,26 +159,28 @@ Section world_ghost_theory.
     - iDestruct (region_open_next_temp_pwl with "[$Hr $Hrel $Hsts]")
         as "(%w & Hr & Hsts & Hstd_sta & Ha & Hp & Hmono & HΦ)" ;[set_solver|..]; eauto.
       iFrame.
-      rewrite decide_True; eauto.
+      rewrite /mono_temporary decide_True; eauto.
     - iDestruct (region_open_next_temp_nwl with "[$Hr $Hrel $Hsts]")
         as "(%w & Hr & Hsts & Hstd_sta & Ha & Hp & Hmono & HΦ)" ;[set_solver|..]; eauto.
       iFrame.
-      destruct (isDL p) eqn:Hp_DL; [rewrite decide_True | rewrite decide_False]; eauto.
+      rewrite /mono_temporary ; destruct (isDL p) eqn:Hp_DL; [rewrite decide_True | rewrite decide_False]; eauto.
       rewrite Hp_WL; intros []; done.
   Qed.
 
-  Lemma close_temporary
+  Lemma close_world_interp_temporary
     (W : WORLD) (C : CmptName) (s : list Addr) (a : Addr) (p : Perm) Φ (w : Word)
     `{forall WCv, Persistent (Φ WCv)}:
     a ∉ s ->
     world_interp_open W C ({[ a ]} ∪ s) -∗
     rel C a p Φ -∗
     sts_state_std C a Temporary -∗
-    TmpRes W C a p Φ w -∗
+    TmpRes W C a p Φ w
+    -∗
     world_interp_open W C s ∗ rel C a p Φ.
   Proof.
     rewrite world_interp_open_eq /world_interp_open_def.
     iIntros (Ha) "[Hr Hsts] #Hrel Hstd_sta (HpO & Ha & HΦ & Hmono)".
+    rewrite /mono_temporary.
     destruct (isWL p) eqn:Hp_WL.
     - iDestruct (region_close_next_temp_pwl with "[Hr Hrel Hstd_sta HpO Ha HΦ Hmono]") as "Hr"
       ; eauto; iFrame "∗ #".
@@ -131,13 +192,15 @@ Section world_ghost_theory.
       + destruct ( decide (false = true ∨ true = true) ) as [ Hdex | Hdec ]; auto.
   Qed.
 
-  Lemma open_permanent (W : WORLD) (C : CmptName) (s : list Addr) (a : Addr) (p : Perm) Φ :
+  Lemma open_world_interp_permanent (W : WORLD) (C : CmptName) (s : list Addr) (a : Addr) (p : Perm) Φ :
     a ∉ s ->
     (std W) !! a = Some Permanent ->
     world_interp_open W C s -∗
     rel C a p Φ
     -∗
-    world_interp_open W C ({[ a ]} ∪ s) ∗ sts_state_std C a Permanent ∗ ▷ (∃ w, PermRes W C a p Φ w).
+    world_interp_open W C ({[ a ]} ∪ s) ∗
+    sts_state_std C a Permanent ∗
+    ▷ (∃ w, PermRes W C a p Φ w).
   Proof.
     rewrite world_interp_open_eq /world_interp_open_def.
     iIntros (Ha HWa) "[Hr Hsts] Hrel".
@@ -146,13 +209,14 @@ Section world_ghost_theory.
     iFrame.
   Qed.
 
-  Lemma close_permanent (W : WORLD) (C : CmptName)
+  Lemma close_world_interp_permanent (W : WORLD) (C : CmptName)
     (s : list Addr) (a : Addr) (p : Perm) Φ (w : Word) `{forall WCv, Persistent (Φ WCv)}:
     a ∉ s ->
     world_interp_open W C ({[ a ]} ∪ s) -∗
     rel C a p Φ -∗
     sts_state_std C a Permanent -∗
-    PermRes W C a p Φ w -∗
+    PermRes W C a p Φ w
+    -∗
     world_interp_open W C s ∗ rel C a p Φ.
   Proof.
     rewrite world_interp_open_eq /world_interp_open_def.
@@ -161,7 +225,47 @@ Section world_ghost_theory.
     ; eauto; iFrame "∗ #".
   Qed.
 
-  Lemma revoke_world (W : WORLD) (C : CmptName) (s : list Addr) :
+  Lemma open_world_interp
+    (W : WORLD) (C : CmptName) (a : Addr) (p : Perm) (φ : Vc) (ρ : region_type) :
+    ρ = Temporary ∨ ρ = Permanent →
+    (std W) !! a = Some ρ →
+    rel C a p φ -∗
+    world_interp W C
+    -∗
+    world_interp_open W C [a] ∗
+    sts_state_std C a ρ ∗
+    ▷ (∃ v, WorldRes W C a p φ v ρ).
+  Proof.
+    rewrite world_interp_eq /world_interp_def.
+    rewrite world_interp_open_eq /world_interp_open_def.
+    iIntros (Hne Htemp) "Hrel [Hreg Hfull]".
+    iDestruct (region_open with "[$Hrel $Hreg $Hfull]") as (v) "(Hr & Hfull & Hstate & Hl & Hp & Hmono & φ)"; eauto.
+    rewrite -(mono_invariant_eq C p φ v ρ).
+    rewrite -region_open_prepare; iFrame.
+  Qed.
+
+  Lemma close_world_interp
+    (W : WORLD) (C : CmptName) (a : Addr) (p : Perm) (φ : Vc) (v : Word)
+    (ρ : region_type) `{forall Wv, Persistent (φ Wv)} :
+    ρ = Temporary ∨ ρ = Permanent →
+
+    world_interp_open W C [a] -∗
+    sts_state_std C a ρ -∗
+    rel C a p φ -∗
+    WorldRes W C a p φ v ρ
+    -∗
+    world_interp W C.
+  Proof.
+    rewrite world_interp_eq /world_interp_def.
+    rewrite world_interp_open_eq /world_interp_open_def.
+    rewrite -region_open_prepare.
+    iIntros (Hρ) "[Hreg_open $] Hstate Hrel (Hp&Ha&Hφ&Hmono)".
+    rewrite (mono_invariant_eq C p φ v ρ).
+    iApply (region_close with "[$Hstate $Hreg_open $Ha $Hp $Hmono $Hφ $Hrel]"); eauto.
+  Qed.
+
+
+  Lemma world_interp_revoke_world (W : WORLD) (C : CmptName) (s : list Addr) :
     NoDup s →
     ( ∀ a, a ∈ s ↔ (std W) !! a = Some Temporary ) →
     world_interp W C
@@ -180,6 +284,7 @@ Section world_ghost_theory.
     cbn.
     iDestruct "Htmp" as (w) "(HpO & Ha & Hmono & HΦ)".
     iFrame.
+    rewrite /mono_temporary.
     destruct (isWL p) eqn:Hp_WL.
     - destruct (decide (true = true ∨ isDL p = true)) as [Hdec | Hdec]; auto.
       exfalso; apply Hdec; left; done.
@@ -190,7 +295,7 @@ Section world_ghost_theory.
         destruct Hdec as []; done.
   Qed.
 
-  Lemma restore_world (W W' : WORLD) (C : CmptName) (s : list Addr) :
+  Lemma world_interp_restore_world (W W' : WORLD) (C : CmptName) (s : list Addr) :
     related_sts_pub_world W (reinstate W' s) →
     world_interp W' C -∗
     RevokedRes W C s
@@ -205,6 +310,7 @@ Section world_ghost_theory.
       iApply (big_sepL_impl with "HrevokedRes").
       iModIntro ; iIntros (k a Hk) "(%p & %Φ & Hrel & H & (%wa & HpO & Ha & HΦ & Hmono))".
       iFrame; iFrame.
+      rewrite /mono_temporary.
       destruct (isWL p) eqn:Hp_WL.
       - destruct (decide (true = true ∨ isDL p = true)) as [Hdec | Hdec]; auto.
         exfalso; apply Hdec; left; done.
@@ -215,6 +321,27 @@ Section world_ghost_theory.
           destruct Hdec as []; done.
     }
     iMod (monotone_close_list_region with "[%] [$Hsts $Hr $H]") as "[$ $]"; eauto.
+  Qed.
+
+  Lemma PermRes_acc (W : WORLD) (C : CmptName) (a : Addr) (p : Perm) (Φ : Vc) (w : Word) :
+    PermRes W C a p Φ w -∗
+    ( a ↦ₐ w ∗ Φ (W,C,w) ) ∗
+    ( ( a ↦ₐ w ∗ Φ (W,C,w) ) -∗ PermRes W C a p Φ w ).
+  Proof.
+    iIntros "(#Hp&Ha&HΦ&#Hmono)".
+    iSplitL "Ha HΦ"; iFrame.
+    iIntros "[Ha HΦ]"; iFrame "∗#".
+  Qed.
+
+  Lemma PermRes_acc' (W : WORLD) (C : CmptName) (a : Addr) (p : Perm) (Φ : Vc) (w : Word) :
+    PermRes W C a p Φ w -∗
+    ( a ↦ₐ w ∗ Φ (W,C,w) ∗ mono_permanent C Φ w ) ∗
+    ( ∀ w', ( a ↦ₐ w' ∗ Φ (W,C,w') ∗ mono_permanent C Φ w' ) -∗ PermRes W C a p Φ w' ).
+  Proof.
+    iIntros "(#Hp&Ha&HΦ&Hmono)".
+    iSplitL "Ha HΦ Hmono"; iFrame.
+    iIntros (w') "($&$&$)".
+    done.
   Qed.
 
 End world_ghost_theory.
